translator dir builds again

translator/ml_monadScript.sml
@@ -7,7 +7,7 @@ open ml_translatorTheory;
 open ml_translatorLib;
 
 open hol_kernelTheory;
-open stringTheory;
+open stringTheory listTheory;
 open MiniMLTheory;
 
 infix \\ val op \\ = op THEN;
@@ -61,6 +61,36 @@ val res = translate string_ge_def;
 (* construct type refinement invariants *)
 
 val _ = register_type ``:hol_type``;
+
+val MEM_hol_type_size = prove(
+  ``!ts t. MEM t ts ==> hol_type_size t < hol_type1_size ts``,
+  Induct \\ FULL_SIMP_TAC (srw_ss()) [] \\ REPEAT STRIP_TAC \\ RES_TAC
+  \\ EVAL_TAC \\ FULL_SIMP_TAC std_ss [] \\ DECIDE_TAC);
+
+val hol_type_ind = store_thm("hol_type_ind",
+  ``(!s ts. (!t. MEM t ts ==> P t) ==> P (Tyapp s ts)) /\
+    (!v. P (Tyvar v)) ==> !x. P x``,
+  REPEAT STRIP_TAC \\ completeInduct_on `hol_type_size x`
+  \\ REPEAT STRIP_TAC \\ FULL_SIMP_TAC std_ss [PULL_FORALL]
+  \\ Cases_on `x` \\ FULL_SIMP_TAC std_ss []
+  \\ Q.PAT_ASSUM `!x1 x2. bb` MATCH_MP_TAC
+  \\ REPEAT STRIP_TAC \\ Q.PAT_ASSUM `!x.bbb` MATCH_MP_TAC
+  \\ EVAL_TAC \\ IMP_RES_TAC MEM_hol_type_size \\ DECIDE_TAC);
+
+val HOL_TYPE_TYPE_def = fetch "-" "HOL_TYPE_TYPE_def"
+
+val EqualityType_HOL_TYPE = prove(
+  ``EqualityType HOL_TYPE_TYPE``,
+  SIMP_TAC std_ss [EqualityType_def] \\ STRIP_TAC THEN1
+   (HO_MATCH_MP_TAC hol_type_ind
+    \\ FULL_SIMP_TAC std_ss [HOL_TYPE_TYPE_def]
+    \\ REPEAT STRIP_TAC
+    \\ FULL_SIMP_TAC std_ss [no_closures_def,EVERY_DEF]
+    \\ cheat)
+  \\ HO_MATCH_MP_TAC hol_type_ind \\ REPEAT STRIP_TAC \\ Cases_on `x2`
+  \\ FULL_SIMP_TAC (srw_ss()) [HOL_TYPE_TYPE_def] \\ cheat)
+  |> store_eq_thm;
+
 val _ = register_type ``:term``;
 val _ = register_type ``:thm``;
 
@@ -71,6 +101,9 @@ val _ = register_type ``:thm``;
   fetch "-" "TERM_TYPE_def";
   fetch "-" "THM_TYPE_def";
 *)
+
+val U_TYPE_def = Define `
+  U_TYPE (u:unit) v = (v = Litv Unit)`;
 
 (* definition of EvalM *)
 
@@ -84,15 +117,18 @@ val HOL_STORE_def = Define `
 
 val EvalM_def = Define `
   EvalM env exp P <=>
-    !s refs. HOL_STORE s refs ==> ?res. evaluate' s env exp res /\ P (s,refs) res`;
+    !s refs. HOL_STORE s refs ==>
+             ?s2 res refs2. evaluate' s env exp (s2,res) /\
+                            P (refs,s) (refs2,s2,res) /\ HOL_STORE s2 refs2`;
 
 (* refinement invariant for ``:'a M`` *)
 
 val HOL_MONAD_def = Define `
-  HOL_MONAD (a:'a->v->bool) (x:'a M) (s1:store,state) (res: (store # v result)) =
-    case (x state, res) of
-      ((HolRes y, state), (s2, Rval v)) => HOL_STORE s2 state /\ a y v
-    | ((HolErr e, state), (s2, Rerr _)) => HOL_STORE s2 state
+  HOL_MONAD (a:'a->v->bool) (x:'a M) (state1:hol_refs,s1:store)
+                                     (state2:hol_refs,s2:store,res) =
+    case (x state1, res) of
+      ((HolRes y, state), Rval v) => (state = state2) /\ a y v
+    | ((HolErr e, state), Rerr _) => (state = state2)
     | _ => F`
 
 (* return *)
@@ -101,7 +137,7 @@ val EvalM_return = store_thm("EvalM_return",
   ``Eval env exp (a x) ==>
     EvalM env exp (HOL_MONAD a (ex_return x))``,
   SIMP_TAC std_ss [Eval_def,EvalM_def,HOL_MONAD_def,ex_return_def]
-  \\ REPEAT STRIP_TAC \\ Q.EXISTS_TAC `s,(Rval (res))`
+  \\ REPEAT STRIP_TAC \\ Q.LIST_EXISTS_TAC [`s`,`Rval res`,`refs`]
   \\ FULL_SIMP_TAC (srw_ss()) [evaluate'_empty_store_IMP]);
 
 (* bind *)
@@ -114,34 +150,215 @@ val EvalM_bind = store_thm("EvalM_bind",
   \\ FULL_SIMP_TAC std_ss [PULL_EXISTS] \\ RES_TAC
   \\ Cases_on `x refs` \\ Cases_on `q`
   \\ Cases_on `res` \\ FULL_SIMP_TAC (srw_ss()) [] THEN1
-   (Cases_on `r'` \\ FULL_SIMP_TAC (srw_ss()) [] \\ REPEAT STRIP_TAC
+   (FULL_SIMP_TAC (srw_ss()) [] \\ REPEAT STRIP_TAC
     \\ Q.MATCH_ASSUM_RENAME_TAC `x refs = (HolRes res1,r)` []
     \\ Q.MATCH_ASSUM_RENAME_TAC `evaluate' s env e1 (q,Rval (state1))` []
     \\ FULL_SIMP_TAC std_ss [PULL_FORALL]
     \\ Q.PAT_ASSUM `!xx.bbb` (MP_TAC o Q.SPECL [`res1`,`state1`,`q`,`r`])
     \\ FULL_SIMP_TAC std_ss [] \\ STRIP_TAC
-    \\ Q.EXISTS_TAC `res` \\ REPEAT STRIP_TAC THEN1
+    \\ Q.LIST_EXISTS_TAC [`s2'`,`res`,`refs2'`]
+    \\ FULL_SIMP_TAC std_ss [] \\ STRIP_TAC THEN1
      (ONCE_REWRITE_TAC [evaluate'_cases]
       \\ FULL_SIMP_TAC (srw_ss()) [] \\ DISJ1_TAC
       \\ Q.LIST_EXISTS_TAC [`state1`,`q`] \\ ASM_SIMP_TAC std_ss [bind_def])
     \\ FULL_SIMP_TAC (srw_ss()) [ex_bind_def])
   THEN1
-   (Cases_on `r'` \\ FULL_SIMP_TAC (srw_ss()) [] \\ REPEAT STRIP_TAC
+   (FULL_SIMP_TAC (srw_ss()) [] \\ REPEAT STRIP_TAC
     \\ Q.MATCH_ASSUM_RENAME_TAC `x refs = (HolErr res1,r)` []
     \\ Q.MATCH_ASSUM_RENAME_TAC `evaluate' s env e1 (q,Rerr (state1))` []
     \\ FULL_SIMP_TAC std_ss [PULL_FORALL]
-    \\ Q.EXISTS_TAC `(q,Rerr state1)` \\ STRIP_TAC
+    \\ Q.LIST_EXISTS_TAC [`q`,`Rerr state1`,`refs2`]
+    \\ FULL_SIMP_TAC std_ss [] \\ STRIP_TAC
     THEN1 (ONCE_REWRITE_TAC [evaluate'_cases] \\ FULL_SIMP_TAC (srw_ss()) [])
     \\ FULL_SIMP_TAC (srw_ss()) [ex_bind_def]));
 
+(* function abstraction and application *)
+
+val any_evaluate_closure_def = Define `
+  any_evaluate_closure (s1,input) cl (s2,output) =
+     ?env exp.
+       (do_app s1 ARB Opapp cl input = SOME (s1,env,exp)) /\
+       evaluate' s1 env exp (s2,output)`
+
+val _ = type_abbrev("H",``:'a -> hol_refs # store ->
+                                 hol_refs # store # v result -> bool``);
+
+val PURE_def = Define `
+  PURE a x (refs1:hol_refs,s1:store) (refs2,s2,res) =
+    ?v:v. (res = Rval v) /\ (refs1 = refs2) /\ (s1 = s2) /\ a x v`;
+
+val ArrowP_def = Define `
+  (ArrowP : 'a H -> 'b H -> ('a -> 'b) -> v -> bool) a b f c =
+     !x refs1 s1 refs2 s2 res.
+       a x (refs1,s1) (refs2,s2,res) /\ HOL_STORE s1 refs1 ==>
+       (refs2 = refs1) /\ (s2 = s1) /\
+       ?v s3 res3 refs3.
+         (res = Rval v) /\ any_evaluate_closure (s2,v) c (s3,res3) /\
+         b (f x) (refs1,s1) (refs3,s3,res3) /\ HOL_STORE s3 refs3`;
+
+val ArrowM_def = Define `
+  (ArrowM : 'a H -> 'b H -> ('a -> 'b) H) a b = PURE (ArrowP a b)`;
+
+val _ = add_infix("-M->",400,HOLgrammars.RIGHT)
+val _ = overload_on ("-M->",``ArrowM``)
+
+val EvalM_ArrowM = store_thm("Evalm_ArrowM",
+  ``EvalM env x1 ((a -M-> b) f) ==>
+    EvalM env x2 (a x) ==>
+    EvalM env (App Opapp x1 x2) (b (f x))``,
+  SIMP_TAC std_ss [EvalM_def,ArrowM_def,ArrowP_def,PURE_def] \\ REPEAT STRIP_TAC
+  \\ FULL_SIMP_TAC std_ss [PULL_EXISTS]
+  \\ ONCE_REWRITE_TAC [evaluate'_cases] \\ SIMP_TAC (srw_ss()) []
+  \\ Q.PAT_ASSUM `!s. bbb` MP_TAC
+  \\ Q.PAT_ASSUM `!s. bbb` (MP_TAC o Q.SPECL [`s`,`refs`])
+  \\ FULL_SIMP_TAC std_ss [] \\ STRIP_TAC \\ STRIP_TAC
+  \\ `!x. evaluate' s env x1 x = (x = (s,Rval v))` by
+       METIS_TAC [big_exp_determ']
+  \\ FULL_SIMP_TAC (srw_ss()) [] \\ POP_ASSUM (K ALL_TAC)
+  \\ Q.PAT_ASSUM `!s. bbb` (MP_TAC o Q.SPECL [`s`,`refs`])
+  \\ FULL_SIMP_TAC std_ss [] \\ STRIP_TAC
+  \\ RES_TAC \\ POP_ASSUM (K ALL_TAC)
+  \\ NTAC 4 (POP_ASSUM (K ALL_TAC))
+  \\ `!x. evaluate' s env x2 x = (x = (s2,res))` by
+       METIS_TAC [big_exp_determ']
+  \\ FULL_SIMP_TAC (srw_ss()) [] \\ POP_ASSUM (K ALL_TAC)
+  \\ Q.LIST_EXISTS_TAC [`s3`,`res3`,`refs3`] \\ FULL_SIMP_TAC std_ss []
+  \\ DISJ1_TAC \\ FULL_SIMP_TAC std_ss [any_evaluate_closure_def]
+  \\ FULL_SIMP_TAC (srw_ss()) [do_app_def] \\ METIS_TAC []);
+
+val EvalM_Fun = store_thm("EvalM_Fun",
+  ``(!v x. a x v ==> EvalM ((name,v)::env) body (b (f x))) ==>
+    EvalM env (Fun name body) ((PURE a -M-> b) f)``,
+  SIMP_TAC std_ss [EvalM_def,ArrowM_def,ArrowP_def,PURE_def]
+  \\ REPEAT STRIP_TAC
+  \\ ONCE_REWRITE_TAC [evaluate'_cases] \\ SIMP_TAC (srw_ss()) []
+  \\ FULL_SIMP_TAC (srw_ss()) [PULL_EXISTS,PULL_FORALL]
+  \\ SIMP_TAC (srw_ss()) [any_evaluate_closure_def,do_app_def,bind_def]
+  \\ METIS_TAC []);
+
+val Eval_Fun_Eq = store_thm("Eval_Fun_Eq",
+  ``(!v. a x v ==> EvalM ((name,v)::env) body (b (f x))) ==>
+    EvalM env (Fun name body) ((PURE (Eq a x) -M-> b) f)``,
+  SIMP_TAC std_ss [EvalM_def,ArrowM_def,ArrowP_def,PURE_def,Eq_def]
+  \\ REPEAT STRIP_TAC
+  \\ ONCE_REWRITE_TAC [evaluate'_cases] \\ SIMP_TAC (srw_ss()) []
+  \\ FULL_SIMP_TAC (srw_ss()) [PULL_EXISTS,PULL_FORALL]
+  \\ SIMP_TAC (srw_ss()) [any_evaluate_closure_def,do_app_def,bind_def]
+  \\ METIS_TAC []);
+
+(* Eq simps *)
+
+val EvalM_FUN_FORALL = store_thm("EvalM_FUN_FORALL",
+  ``(!x. EvalM env exp (PURE (p x) f)) ==>
+    EvalM env exp (PURE (FUN_FORALL x. p x) f)``,
+  SIMP_TAC std_ss [EvalM_def,Eq_def,PURE_def] \\ REPEAT STRIP_TAC
+  \\ FULL_SIMP_TAC std_ss [AppReturns_def,FUN_FORALL,PULL_EXISTS]
+  \\ RES_TAC \\ POP_ASSUM (STRIP_ASSUME_TAC o Q.SPEC `ARB`)
+  \\ Q.EXISTS_TAC `v` \\ FULL_SIMP_TAC std_ss [] \\ REPEAT STRIP_TAC
+  \\ RES_TAC \\ POP_ASSUM MP_TAC
+  \\ `!x. evaluate' s env exp x = (x = (s,Rval v))` by METIS_TAC [big_exp_determ']
+  \\ FULL_SIMP_TAC (srw_ss()) []);
+
+val EvalM_FUN_FORALL_EQ = store_thm("EvalM_FUN_FORALL_EQ",
+  ``(!x. EvalM env exp (PURE (p x) f)) =
+    EvalM env exp (PURE (FUN_FORALL x. p x) f)``,
+  REPEAT STRIP_TAC \\ EQ_TAC \\ FULL_SIMP_TAC std_ss [EvalM_FUN_FORALL]
+  \\ EVAL_TAC \\ FULL_SIMP_TAC std_ss [FUN_FORALL] \\ METIS_TAC []);
+
+val M_FUN_FORALL_PUSH1 = prove(
+  ``(FUN_FORALL x. ArrowP a (PURE (b x))) = (ArrowP a (PURE (FUN_FORALL x. b x)))``,
+  FULL_SIMP_TAC std_ss [ArrowP_def,FUN_EQ_THM,AppReturns_def,FUN_FORALL,
+    Eval_def,any_evaluate_closure_def,PURE_def] \\ REPEAT STRIP_TAC \\ REVERSE EQ_TAC
+  THEN1 METIS_TAC [evaluate_11_Rval]
+  \\ REPEAT STRIP_TAC
+  \\ FULL_SIMP_TAC std_ss [PULL_FORALL] \\ RES_TAC
+  \\ POP_ASSUM (fn th => STRIP_ASSUME_TAC (Q.SPEC `ARB` th) THEN ASSUME_TAC th)
+  \\ FULL_SIMP_TAC std_ss [] \\ POP_ASSUM MP_TAC
+  \\ Q.PAT_ASSUM `s2 = s3` ASSUME_TAC \\ FULL_SIMP_TAC (srw_ss()) []
+  \\ `!x. evaluate' s3 env exp x = (x = (s3,Rval v))`
+       by METIS_TAC [big_exp_determ'] \\ FULL_SIMP_TAC std_ss []
+  \\ FULL_SIMP_TAC (srw_ss()) [PULL_EXISTS]
+  \\ REPEAT STRIP_TAC \\ Q.LIST_EXISTS_TAC [`refs3`,`v`]
+  \\ FULL_SIMP_TAC std_ss []) |> GEN_ALL;
+
+val M_FUN_FORALL_PUSH2 = prove(
+  ``(FUN_FORALL x. ArrowP ((PURE (a x))) b) =
+    (ArrowP (PURE (FUN_EXISTS x. a x)) b)``,
+  FULL_SIMP_TAC std_ss [ArrowP_def,FUN_EQ_THM,AppReturns_def,
+    FUN_FORALL,FUN_EXISTS,PURE_def] \\ METIS_TAC []) |> GEN_ALL;
+
+val FUN_EXISTS_Eq = prove(
+  ``(FUN_EXISTS x. Eq a x) = a``,
+  SIMP_TAC std_ss [FUN_EQ_THM,FUN_EXISTS,Eq_def]) |> GEN_ALL;
+
+val M_FUN_QUANT_SIMP = save_thm("M_FUN_QUANT_SIMP",
+  LIST_CONJ [FUN_EXISTS_Eq,M_FUN_FORALL_PUSH1,M_FUN_FORALL_PUSH2]);
+
+(*
+val th = mk_thm([],
+  ``EvalM env exp ((PURE (Eq NUM m) -M-> PURE (Eq (ArrowP (PURE NUM) (HOL_MONAD NUM)) n) -M-> HOL_MONAD NUM) f)``)
+  |> REWRITE_RULE [ArrowM_def]
+  |> Q.GEN `m` |> HO_MATCH_MP EvalM_FUN_FORALL
+  |> Q.GEN `n` |> HO_MATCH_MP EvalM_FUN_FORALL
+  |> SIMP_RULE std_ss [M_FUN_QUANT_SIMP]
+  |> REWRITE_RULE [GSYM ArrowM_def]
+*)
+
+(* failwith *)
+
+val EvalM_failwith = store_thm("EvalM_failwith",
+  ``!x a. EvalM env (Raise (Int_error 0)) (HOL_MONAD a (failwith x))``,
+  SIMP_TAC (srw_ss()) [Eval_def,EvalM_def,HOL_MONAD_def,failwith_def]
+  \\ ONCE_REWRITE_TAC [evaluate'_cases] \\ SIMP_TAC (srw_ss()) [] );
+
+(* read and update refs *)
+
+val get_the_axioms_thm = prove(
+  ``(lookup "the_axioms" env = SOME (Loc 2)) ==>
+    EvalM env (Uapp Deref (Var "the_axioms"))
+      (HOL_MONAD (LIST_TYPE THM_TYPE) get_the_axioms)``,
+  SIMP_TAC std_ss [EvalM_def]
+  \\ ONCE_REWRITE_TAC [evaluate'_cases] \\ SIMP_TAC (srw_ss()) []
+  \\ ONCE_REWRITE_TAC [evaluate'_cases] \\ SIMP_TAC (srw_ss()) []
+  \\ SIMP_TAC (srw_ss()) [do_uapp_def,store_lookup_def]
+  \\ REPEAT STRIP_TAC \\ FULL_SIMP_TAC std_ss [HOL_STORE_def]
+  \\ `2 < LENGTH s` by DECIDE_TAC
+  \\ FULL_SIMP_TAC std_ss []
+  \\ Q.LIST_EXISTS_TAC [`s`,`Rval (EL 2 s)`,`refs`]
+  \\ FULL_SIMP_TAC std_ss []
+  \\ FULL_SIMP_TAC (srw_ss()) [HOL_MONAD_def,get_the_axioms_def]);
+
+val set_the_axioms_thm = prove(
+  ``Eval env exp (LIST_TYPE THM_TYPE x) ==>
+    (lookup "the_axioms" env = SOME (Loc 2)) ==>
+    EvalM env (App Opassign (Var "the_axioms") exp)
+      ((HOL_MONAD U_TYPE) (set_the_axioms x))``,
+  SIMP_TAC std_ss [EvalM_def]
+  \\ ONCE_REWRITE_TAC [evaluate'_cases] \\ SIMP_TAC (srw_ss()) []
+  \\ SIMP_TAC (srw_ss()) [Once evaluate'_cases]
+  \\ SIMP_TAC std_ss [Eval_def] \\ REPEAT STRIP_TAC
+  \\ `evaluate' s env exp (s,Rval res)` by METIS_TAC [evaluate'_empty_store_IMP]
+  \\ `!x. evaluate' s env exp x = (x = (s,Rval res))` by
+       METIS_TAC [big_exp_determ']
+  \\ FULL_SIMP_TAC (srw_ss()) [] \\ SIMP_TAC (srw_ss()) [Once do_app_def]
+  \\ SIMP_TAC (srw_ss()) [Once evaluate'_cases]
+  \\ Q.LIST_EXISTS_TAC [`store_assign 2 res s`,`Rval (Litv Unit)`,
+       `refs with the_axioms := x`] \\ FULL_SIMP_TAC std_ss []
+  \\ REVERSE STRIP_TAC THEN1
+   (FULL_SIMP_TAC std_ss [HOL_STORE_def,store_assign_def,EL_LUPDATE]
+    \\ FULL_SIMP_TAC (srw_ss()) [HOL_STORE_def,store_assign_def,EL_LUPDATE]
+    \\ SRW_TAC [] [] \\ `F` by DECIDE_TAC)
+  \\ FULL_SIMP_TAC (srw_ss()) [HOL_MONAD_def,set_the_axioms_def]
+  \\ EVAL_TAC);
+
 (* some pure functions *)
 
+val res = translate listTheory.MAP;
 val res = translate MEMBER_def;
 val res = translate listTheory.EVERY_DEF;
 val res = translate listTheory.EXISTS_DEF;
 val res = translate listTheory.FILTER;
 val res = translate listTheory.APPEND;
-val res = translate listTheory.MAP;
 val res = translate (subset_def |> REWRITE_RULE [MEMBER_INTRO]);
 val res = translate (subtract_def |> REWRITE_RULE [MEMBER_INTRO]);
 val res = translate (insert_def |> REWRITE_RULE [MEMBER_INTRO]);
